fix: make `elab_as_elim` eagerly elaborate arguments for parameters appearing in the types of targets
The `elab_as_elim` elaborator eagerly elaborates arguments that can help with elaborating the motive, however it does not include the transitive closure of parameters that appear in types of parameters appearing in ... types of targets.

This leads to counter-intuitive behavior where arguments supplied to the eliminator may have postponed elaboration, causing motives to be type incorrect for under-applied eliminators such as the following:

```lean
class IsEmpty (α : Sort u) : Prop where
  protected false : α → False

@[elab_as_elim]
def isEmptyElim [IsEmpty α] {p : α → Sort _} (a : α) : p a :=
  (IsEmpty.false a).elim

example {α : Type _} [IsEmpty α] :
  id (α → False) := isEmptyElim (α := α)
```

The issue is that when `isEmptyElim (α := α)` is computing its motive, the value of the argument `α` is still an assignable metavariable. Now, this argument is among those that are eagerly elaborated since it appears as the type of the target `a`.

This PR also contains some other fixes:
* When underapplied, does unification when instantiating foralls in the expected type.
* When overapplied, type checks the generalized-and-reverted expected type.
* When collecting targets, collects them in the correct order.

This is a followup to #4722, which exposed the eagerness issue.

src/Lean/Elab/App.lean
@@ -5,6 +5,7 @@ Authors: Leonardo de Moura
 -/
 prelude
 import Lean.Util.FindMVar
+import Lean.Util.CollectFVars
 import Lean.Parser.Term
 import Lean.Meta.KAbstract
 import Lean.Meta.Tactic.ElimInfo
@@ -711,6 +712,12 @@ structure Context where
   ```
   theorem Eq.subst' {α} {motive : α → Prop} {a b : α} (h : a = b) : motive a → motive b
   ```
+  For another example, the term `isEmptyElim (α := α)` is an underapplied eliminator, and it needs
+  argument `α` to be elaborated eagerly to create a type correct motive.
+  ```
+  def isEmptyElim [IsEmpty α] {p : α → Sort _} (a : α) : p a := ...
+  example {α : Type _} [IsEmpty α] : id (α → False) := isEmptyElim (α := α)
+  ```
   -/
   extraArgsPos : Array Nat
 
@@ -725,7 +732,7 @@ structure State where
   /-- User-provided arguments that still have to be processed. -/
   args         : List Arg
   /-- Discriminants processed so far. -/
-  discrs       : Array Expr := #[]
+  discrs       : Array (Option Expr)
   /-- Instance implicit arguments collected so far. -/
   instMVars    : Array MVarId := #[]
   /-- Position of the next argument to be processed. We use it to decide whether the argument is the motive or a discriminant. -/
@@ -742,10 +749,7 @@ def mkMotive (discrs : Array Expr) (expectedType : Expr): MetaM Expr := do
     let motiveBody ← kabstract motive discr
     /- We use `transform (usedLetOnly := true)` to eliminate unnecessary let-expressions. -/
     let discrType ← transform (usedLetOnly := true) (← instantiateMVars (← inferType discr))
-    let motive := Lean.mkLambda (← mkFreshBinderName) BinderInfo.default discrType motiveBody
-    unless (← isTypeCorrect motive) do
-      throwError "failed to elaborate eliminator, motive is not type correct:{indentD motive}"
-    return motive
+    return Lean.mkLambda (← mkFreshBinderName) BinderInfo.default discrType motiveBody
 
 /-- If the eliminator is over-applied, we "revert" the extra arguments. -/
 def revertArgs (args : List Arg) (f : Expr) (expectedType : Expr) : TermElabM (Expr × Expr) :=
@@ -761,7 +765,7 @@ def revertArgs (args : List Arg) (f : Expr) (expectedType : Expr) : TermElabM (E
     return (mkApp f val, mkForall (← mkFreshBinderName) BinderInfo.default valType expectedTypeBody)
 
 /--
-Construct the resulting application after all discriminants have bee elaborated, and we have
+Construct the resulting application after all discriminants have been elaborated, and we have
 consumed as many given arguments as possible.
 -/
 def finalize : M Expr := do
@@ -774,21 +778,36 @@ def finalize : M Expr := do
     let mut f := (← get).f
     if xs.size > 0 then
       assert! (← get).args.isEmpty
-      try
-        expectedType ← instantiateForall expectedType xs
-      catch _ =>
-        throwError "failed to elaborate eliminator, insufficient number of arguments, expected type:{indentExpr expectedType}"
+      for x in xs do
+        expectedType ← whnf expectedType
+        let .forallE _ t b _ := expectedType
+          | throwError "failed to elaborate eliminator, insufficient number of arguments, expected type:{indentExpr (← read).expectedType}"
+        unless ← fullApproxDefEq <| isDefEq t (← inferType x) do
+          throwError "failed to elaborate eliminator, binding domain{indentExpr t}\nis not definitionally equal to{indentExpr (← inferType x)}"
+        expectedType := b.instantiate1 x
     else
-      -- over-application, simulate `revert`
+      -- over-application, simulate `revert` while generalizing
       (f, expectedType) ← revertArgs (← get).args f expectedType
+      unless ← isTypeCorrect expectedType do
+        throwError "failed to elaborate eliminator, after generalizing over-applied arguments, expected type is type incorrect:{indentExpr expectedType}"
     let result := mkAppN f xs
     let mut discrs := (← get).discrs
     let idx := (← get).idx
-    if (← get).discrs.size < (← read).elimInfo.targetsPos.size then
+    if discrs.any Option.isNone then
       for i in [idx:idx + xs.size], x in xs do
-        if (← read).elimInfo.targetsPos.contains i then
-          discrs := discrs.push x
-    let motiveVal ← mkMotive discrs expectedType
+        if let some tidx := (← read).elimInfo.targetsPos.indexOf? i then
+          discrs := discrs.set! tidx x
+    if discrs.any Option.isNone then
+      -- This should not happen.
+      throwError "failed to elaborate eliminator, insufficient number of arguments"
+    trace[Elab.app.elab_as_elim] "xs: {xs}"
+    trace[Elab.app.elab_as_elim] "discrs: {discrs.map Option.get!}"
+    trace[Elab.app.elab_as_elim] "result: {result}"
+    trace[Elab.app.elab_as_elim] "expectedType: {expectedType}"
+    trace[Elab.app.elab_as_elim] "motive: {motive}"
+    let motiveVal ← mkMotive (discrs.map Option.get!) expectedType
+    unless (← isTypeCorrect motiveVal) do
+      throwError "failed to elaborate eliminator, motive is not type correct:{indentD motiveVal}"
     unless (← isDefEq motive motiveVal) do
       throwError "failed to elaborate eliminator, invalid motive{indentExpr motiveVal}"
     synthesizeAppInstMVars (← get).instMVars result
@@ -819,9 +838,9 @@ def getNextArg? (binderName : Name) (binderInfo : BinderInfo) : M (LOption Arg) 
 def setMotive (motive : Expr) : M Unit :=
   modify fun s => { s with motive? := motive }
 
-/-- Push the given expression into the `discrs` field in the state. -/
-def addDiscr (discr : Expr) : M Unit :=
-  modify fun s => { s with discrs := s.discrs.push discr }
+/-- Push the given expression into the `discrs` field in the state, where `i` is which target it is for. -/
+def addDiscr (i : Nat) (discr : Expr) : M Unit :=
+  modify fun s => { s with discrs := s.discrs.set! i discr }
 
 /-- Elaborate the given argument with the given expected type. -/
 private def elabArg (arg : Arg) (argExpectedType : Expr) : M Expr := do
@@ -856,11 +875,11 @@ partial def main : M Expr := do
     let motive ← mkImplicitArg binderType binderInfo
     setMotive motive
     addArgAndContinue motive
-  else if (← read).elimInfo.targetsPos.contains idx then
+  else if let some tidx := (← read).elimInfo.targetsPos.indexOf? idx then
     match (← getNextArg? binderName binderInfo) with
-    | .some arg => let discr ← elabArg arg binderType; addDiscr discr; addArgAndContinue discr
+    | .some arg => let discr ← elabArg arg binderType; addDiscr tidx discr; addArgAndContinue discr
     | .undef => finalize
-    | .none => let discr ← mkImplicitArg binderType binderInfo; addDiscr discr; addArgAndContinue discr
+    | .none => let discr ← mkImplicitArg binderType binderInfo; addDiscr tidx discr; addArgAndContinue discr
   else match (← getNextArg? binderName binderInfo) with
     | .some (.stx stx) =>
       if (← read).extraArgsPos.contains idx then
@@ -922,10 +941,12 @@ def elabAppArgs (f : Expr) (namedArgs : Array NamedArg) (args : Array Arg)
     let expectedType ← instantiateMVars expectedType
     if expectedType.getAppFn.isMVar then throwError "failed to elaborate eliminator, expected type is not available"
     let extraArgsPos ← getElabAsElimExtraArgsPos elimInfo
+    trace[Elab.app.elab_as_elim] "extraArgsPos: {extraArgsPos}"
     ElabElim.main.run { elimInfo, expectedType, extraArgsPos } |>.run' {
       f, fType
       args := args.toList
       namedArgs := namedArgs.toList
+      discrs := mkArray elimInfo.targetsPos.size none
     }
   else
     ElabAppArgs.main.run { explicit, ellipsis, resultIsOutParamSupport } |>.run' {
@@ -955,19 +976,28 @@ where
 
   /--
   Collect extra argument positions that must be elaborated eagerly when using `elab_as_elim`.
-  The idea is that the contribute to motive inference. See comment at `ElamElim.Context.extraArgsPos`.
+  The idea is that they contribute to motive inference. See comment at `ElamElim.Context.extraArgsPos`.
   -/
   getElabAsElimExtraArgsPos (elimInfo : ElimInfo) : MetaM (Array Nat) := do
     forallTelescope elimInfo.elimType fun xs type => do
-      let resultArgs := type.getAppArgs
+      let targets := type.getAppArgs
       let mut extraArgsPos := #[]
-      for i in [:xs.size] do
+      /- Transitive closure of fvars appearing in the motive and the targets. -/
+      let mut motiveFVars : CollectFVars.State := collectFVars {} xs[elimInfo.motivePos]!
+      for arg in targets do
+        motiveFVars := collectFVars motiveFVars (← inferType arg)
+      /- Process arguments in reverse order to transitively collect extra args positions -/
+      for i' in [:xs.size] do
+        let i := xs.size - 1 - i'
         let x := xs[i]!
-        unless elimInfo.targetsPos.contains i do
-          let xType ← inferType x
-          /- We only consider "first-order" types because we can reliably "extract" information from them. -/
-          if isFirstOrder xType
-             && Option.isSome (xType.find? fun e => e.isFVar && resultArgs.contains e) then
+        let xType ← x.fvarId!.getType
+        unless elimInfo.motivePos == i || elimInfo.targetsPos.contains i do
+          if motiveFVars.fvarSet.contains x.fvarId! then
+            extraArgsPos := extraArgsPos.push i
+            motiveFVars := collectFVars motiveFVars xType
+          else if isFirstOrder xType
+                  && Option.isSome (xType.find? fun e => e.isFVar && motiveFVars.fvarSet.contains e.fvarId!) then
+            /- We only consider "first-order" types because we can reliably "extract" information from them. -/
             extraArgsPos := extraArgsPos.push i
       return extraArgsPos
 
@@ -1528,5 +1558,6 @@ builtin_initialize
   registerTraceClass `Elab.app.args (inherited := true)
   registerTraceClass `Elab.app.propagateExpectedType (inherited := true)
   registerTraceClass `Elab.app.finalize (inherited := true)
+  registerTraceClass `Elab.app.elab_as_elim (inherited := true)
 
 end Lean.Elab.Term
